pcuic/theories/PCUICInductives.v
@@ -93,20 +93,20 @@ Lemma branch_type_spec {cf:checker_flags} Σ ind mdecl idecl cdecl pars u p c na
   declared_inductive Σ mdecl ind idecl ->
   forall (omib : on_inductive (lift_typing typing) (Σ, ind_universes mdecl) (inductive_mind ind) mdecl),
   forall (oib : on_ind_body (lift_typing typing) (Σ, ind_universes mdecl) (inductive_mind ind) mdecl (inductive_ind ind) idecl),
-  forall cshape (cs : on_constructor (lift_typing typing) (Σ, ind_universes mdecl) mdecl (inductive_ind ind) idecl (ind_indices oib) cdecl cshape),
+  forall cdecl (cs : on_constructor (lift_typing typing) (Σ, ind_universes mdecl) mdecl (inductive_ind ind) idecl (ind_indices oib) cdecl cdecl),
   branch_type ind mdecl idecl pars u p c cdecl = Some (nargs, bty) ->
-  nargs = context_assumptions cshape.(cshape_args) /\
+  nargs = context_assumptions cdecl.(cstr_args) /\
   forall parsubst, 
   context_subst (subst_instance_context u (PCUICAst.ind_params mdecl)) pars parsubst ->
   let indsubst := (inds (inductive_mind ind) u (ind_bodies mdecl)) in
-  let nargs' := #|cshape.(cshape_args)| in
+  let nargs' := #|cdecl.(cstr_args)| in
   let npars := #|ind_params mdecl| in
   let substargs := (subst_context parsubst 0 
-    (subst_context indsubst npars (map_context (subst_instance_constr u) cshape.(cshape_args)))) in
+    (subst_context indsubst npars (map_context (subst_instance_constr u) cdecl.(cstr_args)))) in
   bty = 
   it_mkProd_or_LetIn substargs
     (mkApps (lift0 nargs' p)
-      (map (subst parsubst nargs' ∘ subst indsubst (nargs' + npars) ∘ subst_instance_constr u) cshape.(cshape_indices) ++ 
+      (map (subst parsubst nargs' ∘ subst indsubst (nargs' + npars) ∘ subst_instance_constr u) cdecl.(cstr_indices) ++ 
        [mkApps (tConstruct ind c u)
          (map (lift0 nargs') pars ++         
           to_extended_list substargs)])).
@@ -365,29 +365,29 @@ Lemma subslet_projs {cf:checker_flags} (Σ : global_env_ext) i mdecl idecl :
   forall (wfΣ : wf Σ.1) 
   (Hdecl : declared_inductive Σ.1 mdecl i idecl),
   let oib := declared_inductive_inv weaken_env_prop_typing wfΣ wfΣ Hdecl in
-  match ind_cshapes oib return Type with
+  match ind_cunivs oib return Type with
   | [cs] => 
     on_projections mdecl (inductive_mind i) (inductive_ind i) 
      idecl (ind_indices oib) cs -> 
      forall Γ t u,
      let indsubst := inds (inductive_mind i) u (ind_bodies mdecl) in
      untyped_subslet Γ
-     (projs_inst i (ind_npars mdecl) (context_assumptions (cshape_args cs)) t)
+     (projs_inst i (ind_npars mdecl) (context_assumptions (cstr_args cs)) t)
      (smash_context []
         (subst_context (inds (inductive_mind i) u (ind_bodies mdecl))
-           #|ind_params mdecl| (subst_instance_context u (cshape_args cs))))
+           #|ind_params mdecl| (subst_instance_context u (cstr_args cs))))
   | _ => True
   end.
 Proof.
   intros wfΣ Hdecl oib.
-  destruct ind_cshapes as [|cs []] eqn:Heq; trivial.
+  destruct ind_cunivs as [|cs []] eqn:Heq; trivial.
   intros onp. simpl. intros Γ t u. 
   rewrite (smash_context_subst []).
   destruct onp.
   assert (#|PCUICEnvironment.ind_projs idecl| >=
-  PCUICEnvironment.context_assumptions (cshape_args cs)). lia.
+  PCUICEnvironment.context_assumptions (cstr_args cs)). lia.
   clear on_projs_all.
-  induction (cshape_args cs) as [|[? [] ?] ?].
+  induction (cstr_args cs) as [|[? [] ?] ?].
   - simpl. constructor.
   - simpl. apply IHc. now simpl in H.
   - simpl. rewrite smash_context_acc /=.
@@ -481,14 +481,14 @@ Lemma on_projections_decl {cf:checker_flags} {Σ mdecl ind idecl cs} :
   on_projections mdecl (inductive_mind ind) (inductive_ind ind) idecl (oib.(ind_indices)) cs ->
   Alli (fun i decl => 
     ∑ pdecl, 
-      (nth_error (ind_projs idecl) (context_assumptions (cshape_args cs) - S i) = Some pdecl))
-    0 (smash_context [] cs.(cshape_args)).
+      (nth_error (ind_projs idecl) (context_assumptions (cstr_args cs) - S i) = Some pdecl))
+    0 (smash_context [] cs.(cstr_args)).
 Proof.
   intros.
   destruct X as [_ _ _ on_projs_all on_projs].
   eapply forall_nth_error_Alli.
   intros.
-  pose proof (snd (nth_error_Some' (ind_projs idecl) (context_assumptions (cshape_args cs) - S i))).
+  pose proof (snd (nth_error_Some' (ind_projs idecl) (context_assumptions (cstr_args cs) - S i))).
   apply X. eapply nth_error_Some_length in H. 
     autorewrite with len in H. simpl in H; lia.
 Qed.
@@ -498,7 +498,7 @@ Lemma declared_projections {cf:checker_flags} {Σ : global_env_ext} {mdecl ind i
   forall (wfΣ : wf Σ.1) (Hdecl : declared_inductive Σ mdecl ind idecl),
   let oib := declared_inductive_inv weaken_env_prop_typing wfΣ wfΣ Hdecl in
   let u := PCUICLookup.abstract_instance (ind_universes mdecl) in
-  match ind_cshapes oib return Type with
+  match ind_cunivs oib return Type with
   | [cs] => 
     on_projections mdecl (inductive_mind ind) (inductive_ind ind) 
       idecl (ind_indices oib) cs -> 
@@ -509,11 +509,11 @@ Lemma declared_projections {cf:checker_flags} {Σ : global_env_ext} {mdecl ind i
             (to_extended_list (smash_context [] (ind_params mdecl)))))::
           smash_context [] (ind_params mdecl)) pdecl.2 * 
       ∑ decl, 
-        (nth_error (smash_context [] (cshape_args cs)) 
-          (context_assumptions (cshape_args cs) - S i) = Some decl) *
+        (nth_error (smash_context [] (cstr_args cs)) 
+          (context_assumptions (cstr_args cs) - S i) = Some decl) *
         wf_local (Σ.1, ind_universes mdecl) 
           (arities_context (ind_bodies mdecl) ,,, 
-            ind_params mdecl ,,, smash_context [] (cshape_args cs)) *
+            ind_params mdecl ,,, smash_context [] (cstr_args cs)) *
         (projection_type mdecl ind i decl.(decl_type) = pdecl.2) *
         (projection_type mdecl ind i decl.(decl_type) = 
             projection_type' mdecl ind  i decl.(decl_type)))%type
@@ -523,7 +523,7 @@ Lemma declared_projections {cf:checker_flags} {Σ : global_env_ext} {mdecl ind i
 Proof.
   intros wfΣ decli oib u.
   set(indb := {| binder_name := _ |}) in *.
-  destruct (ind_cshapes oib) as [|? []] eqn:Heq; try contradiction; auto.
+  destruct (ind_cunivs oib) as [|? []] eqn:Heq; try contradiction; auto.
   intros onps.
   eapply forall_nth_error_Alli.
   set (eos := CoreTactics.the_end_of_the_section).
@@ -547,7 +547,7 @@ Proof.
   rewrite {}onp.
   apply on_projections_decl in onps.
   clearbody oib.
-  assert(projslen : #|ind_projs idecl| = (context_assumptions (cshape_args c))).
+  assert(projslen : #|ind_projs idecl| = (context_assumptions (cstr_args c))).
   { now destruct onProjs. }
   assert (some_proj :#|ind_projs idecl| > 0).
   { destruct isdecl as [ [] []]. now apply nth_error_Some_length in H1. }
@@ -648,7 +648,7 @@ Proof.
   rewrite smash_context_acc in Heq'. 
   rewrite nth_error_app_lt in Heq'.
   autorewrite with len. lia.
-  set (idx := context_assumptions (cshape_args c) - S i) in *.
+  set (idx := context_assumptions (cstr_args c) - S i) in *.
   unshelve epose proof (nth_error_All_local_env (n:=idx) _ wfsargs).
   autorewrite with len. rewrite /lift_context /subst_context !context_assumptions_fold.
   subst idx; lia.
@@ -683,7 +683,7 @@ Proof.
   assert(clarg : closedn (i + #|ind_params mdecl| + #|ind_bodies mdecl|) (decl_type arg)).
   { assert(wf_local (Σ.1, ind_universes mdecl)
       (arities_context (ind_bodies mdecl) ,,, ind_params mdecl ,,, 
-      smash_context [] (cshape_args c))).
+      smash_context [] (cstr_args c))).
     apply All_local_env_app; split; auto.
     now apply All_local_env_app_inv in wfargs as [wfindpars wfargs].
     apply wf_local_rel_smash_context; auto.
@@ -699,9 +699,9 @@ Proof.
   destruct ind as [mind ind]; simpl in *.
   autorewrite with len. simpl.
   revert Hs.
-  assert(context_assumptions (cshape_args c) - S idx = i) as -> by lia.
+  assert(context_assumptions (cstr_args c) - S idx = i) as -> by lia.
   rewrite !context_assumptions_fold.
-  assert(context_assumptions (cshape_args c) - S idx + 1 = S i) as -> by lia.
+  assert(context_assumptions (cstr_args c) - S idx + 1 = S i) as -> by lia.
   intros Hs.
   assert (projection_type mdecl {| inductive_mind := mind; inductive_ind := ind |}
       i (decl_type arg) = 
@@ -716,8 +716,8 @@ Proof.
     { clear. subst projsubst. induction i; simpl; auto.
       f_equal. auto. }
     rewrite /projsubst projs_length.
-    replace (context_assumptions (cshape_args c) - S idx + 1) with
-    (context_assumptions (cshape_args c) - idx) by lia.
+    replace (context_assumptions (cstr_args c) - S idx + 1) with
+    (context_assumptions (cstr_args c) - idx) by lia.
     simpl in idx.
     epose proof (commut_lift_subst_rec _ _ 1 (i + ind_npars mdecl) i).
     rewrite -Nat.add_1_r Nat.add_assoc. erewrite <-H0. 2:lia.
@@ -752,7 +752,7 @@ Proof.
   clear -wfΣ parslen onps projslen some_proj IH Hp2 decli.
   rewrite (smash_context_lift []).
   rewrite (smash_context_subst []).
-  rewrite -(firstn_skipn (S idx) (smash_context [] (cshape_args c))).
+  rewrite -(firstn_skipn (S idx) (smash_context [] (cstr_args c))).
   rewrite subst_context_app lift_context_app subst_context_app.
   autorewrite with len.
   rewrite skipn_all_app_eq.
@@ -760,8 +760,8 @@ Proof.
   rewrite firstn_length_le; auto. rewrite smash_context_length.
   simpl. lia.
   induction i. subst idx.
-  - assert (S (context_assumptions (cshape_args c) - 1) =
-      (context_assumptions (cshape_args c))) as -> by lia.
+  - assert (S (context_assumptions (cstr_args c) - 1) =
+      (context_assumptions (cstr_args c))) as -> by lia.
     rewrite skipn_all2.
     autorewrite with len; simpl; auto.
     constructor.
@@ -769,8 +769,8 @@ Proof.
     intros. eapply (IH i0). lia. auto. 
     forward IHi by lia. simpl in IHi.
     subst idx.
-    destruct (skipn (S (context_assumptions (cshape_args c) - S (S i))) 
-      (smash_context [] (cshape_args c))) eqn:eqargs.
+    destruct (skipn (S (context_assumptions (cstr_args c) - S (S i))) 
+      (smash_context [] (cstr_args c))) eqn:eqargs.
     apply (f_equal (@length _)) in eqargs.
     autorewrite with len in eqargs.
     rewrite skipn_length in eqargs. autorewrite with len. simpl; lia.
@@ -779,14 +779,14 @@ Proof.
     simpl.
     destruct c0 as [? [] ?].
     * simpl in eqargs.
-      pose proof (@smash_context_assumption_context [] (cshape_args c)).
+      pose proof (@smash_context_assumption_context [] (cstr_args c)).
       forward H by constructor.
       eapply assumption_context_skipn in H.
       rewrite -> eqargs in H. elimtype False; inv H.
     * apply skipn_eq_cons in eqargs as [Hnth eqargs].
       constructor.
-      + replace (S (S (context_assumptions (cshape_args c) - S (S i)))) 
-          with (S (context_assumptions (cshape_args c) - S i)) in eqargs by lia.
+      + replace (S (S (context_assumptions (cstr_args c) - S (S i)))) 
+          with (S (context_assumptions (cstr_args c) - S i)) in eqargs by lia.
         rewrite eqargs in IHi. apply IHi.
       + rewrite /lift_decl /=.
         autorewrite with len.
@@ -798,8 +798,8 @@ Proof.
         autorewrite with len in eqargs. simpl in eqargs.
         eapply nth_error_alli in onps; eauto. simpl in onps.
         destruct onps as [pdecl Hnth'].
-        replace ((context_assumptions (cshape_args c) - 
-          S (S (context_assumptions (cshape_args c) - S (S i)))))
+        replace ((context_assumptions (cstr_args c) - 
+          S (S (context_assumptions (cstr_args c) - S (S i)))))
           with i in eqargs, Hnth' by lia. rewrite -eqargs.
         rewrite /lift_decl /subst_decl. simpl.
         autorewrite with len.
@@ -822,8 +822,8 @@ Proof.
           eapply declared_inductive_wf_ext_wk; eauto with pcuic. }
         destruct IH as [isTy [decl [[[nthdecl _] eqpdecl] ptyeq]]].
         move ptyeq at bottom. 
-        replace  (S (context_assumptions (cshape_args c) - S (S i))) with 
-          (context_assumptions (cshape_args c) - S i) in Hnth by lia.
+        replace  (S (context_assumptions (cstr_args c) - S (S i))) with 
+          (context_assumptions (cstr_args c) - S i) in Hnth by lia.
         rewrite nthdecl in Hnth. noconf Hnth. simpl in ptyeq.
         rewrite -eqpdecl. simpl.
         rewrite ptyeq. unfold projection_type'.
@@ -872,7 +872,7 @@ Proof.
   intros onprojs u.
   clearbody oib.
   simpl in *.
-  destruct (ind_cshapes oib) as [|? []]; try contradiction.
+  destruct (ind_cunivs oib) as [|? []]; try contradiction.
   forward onprojs. intuition auto.
   destruct declp as [decli [Hnth Hpars]].
   eapply nth_error_alli in onprojs; eauto.
@@ -883,7 +883,7 @@ Lemma declared_projection_type_and_eq {cf:checker_flags} {Σ : global_env_ext} {
   forall (wfΣ : wf Σ.1) (Hdecl : declared_projection Σ mdecl idecl p pdecl),
   let u := PCUICLookup.abstract_instance (ind_universes mdecl) in
   let oib := declared_inductive_inv weaken_env_prop_typing wfΣ wfΣ (let (x, _) := Hdecl in x) in
-  match ind_cshapes oib return Type with
+  match ind_cunivs oib return Type with
   | [cs] => 
     isType (Σ.1, ind_universes mdecl)
       ((vass {| binder_name := nAnon; binder_relevance := idecl.(ind_relevance) |}
@@ -891,11 +891,11 @@ Lemma declared_projection_type_and_eq {cf:checker_flags} {Σ : global_env_ext} {
             (to_extended_list (smash_context [] (ind_params mdecl)))))::
         smash_context [] (ind_params mdecl)) pdecl.2 *
     ∑ decl, 
-    (nth_error (smash_context [] (cshape_args cs)) 
-      (context_assumptions (cshape_args cs) - S p.2) = Some decl) *
+    (nth_error (smash_context [] (cstr_args cs)) 
+      (context_assumptions (cstr_args cs) - S p.2) = Some decl) *
     (wf_local (Σ.1, ind_universes mdecl) 
         (arities_context (ind_bodies mdecl) ,,, 
-          ind_params mdecl ,,, smash_context [] (cshape_args cs))) *
+          ind_params mdecl ,,, smash_context [] (cstr_args cs))) *
     (projection_type mdecl p.1.1 p.2 decl.(decl_type) = pdecl.2) *
     (projection_type mdecl p.1.1 p.2 decl.(decl_type) = 
       projection_type' mdecl p.1.1 p.2 decl.(decl_type))%type
@@ -909,7 +909,7 @@ Proof.
   intros onprojs u.
   clearbody oib.
   simpl in *.
-  destruct (ind_cshapes oib) as [|? []]; try contradiction.
+  destruct (ind_cunivs oib) as [|? []]; try contradiction.
   forward onprojs. intuition auto.
   destruct declp as [decli [Hnth Hpars]].
   eapply nth_error_alli in onprojs; eauto.
@@ -1128,7 +1128,7 @@ Proof.
   move=> wfΣ decli.
   pose proof (on_declared_projection wfΣ decli) as [onmind onind].
   set (oib := declared_inductive_inv _ _ _ _) in *. clearbody oib.
-  simpl in onind; destruct ind_cshapes as [|? []]; try contradiction.
+  simpl in onind; destruct ind_cunivs as [|? []]; try contradiction.
   destruct onind as [[[_ onps] Hpe] onp].
   move=> cu.
   assert(wfparams : wf_local Σ (subst_instance_context u (ind_params mdecl))).
@@ -1232,7 +1232,7 @@ Proof.
   unfold on_declared_inductive in spargs. simpl in spargs.
   unfold projection_context.
   set (oib := declared_inductive_inv _ _ _ _) in *. clearbody oib.
-  simpl in y. destruct (ind_cshapes oib) as [|cs []]; try contradiction.
+  simpl in y. destruct (ind_cunivs oib) as [|cs []]; try contradiction.
   destruct y as [[[_ onps] ?] ?].
   pose proof (on_projs_noidx _ _ _ _ _ _ onps).
   pose proof (onNpars o).
