replace.sh
@@ -1,4 +1,5 @@
 #/bin/bash
-SED = `which gsed || which sed`
-
-${SED} -i -e s/$1/$2/g */*/*.v
+SED=`which gsed || which sed`
+echo $1
+echo $2
+${SED} -i -e "s/$1/$2/g" */*/*.v
